Rework security notions

Security.thy
@@ -4,7 +4,7 @@ begin
 
 locale security  = rules  
 
-type_synonym ('a,'b) Trace = "('b \<times> 'b) set list" 
+type_synonym ('a,'b) Trace = "('a,'b) basic list" 
 
 context security
 begin
@@ -18,32 +18,6 @@ inductive_set trace :: "(('a,'b,'c) com \<times> ('a,'b) Trace \<times> ('a,'b,'
   | none[intro]: "c \<mapsto>\<^sup>*[] c" 
   | sil[intro]: "c\<^sub>1 \<leadsto> c\<^sub>2 \<Longrightarrow> c\<^sub>2 \<mapsto>\<^sup>*t c\<^sub>3 \<Longrightarrow> c\<^sub>1 \<mapsto>\<^sup>*t c\<^sub>3"
   | gex[intro]: "c\<^sub>1 \<mapsto>[g] c\<^sub>2 \<Longrightarrow> c\<^sub>2 \<mapsto>\<^sup>*t c\<^sub>3 \<Longrightarrow> c\<^sub>1 \<mapsto>\<^sup>*g#t c\<^sub>3"
-
-inductive trace_mem :: "'m \<Rightarrow> 'm rel list  \<Rightarrow> 'm \<Rightarrow> bool" 
-  where
-    [intro]: "trace_mem m [] m" |
-    [intro]: "(m'', m) \<in> g \<Longrightarrow> trace_mem m t m' \<Longrightarrow> trace_mem m'' (g#t) m'"
-
-definition ev :: "('a,'b,'c) com \<Rightarrow> 'b \<Rightarrow> ('a,'b) Trace \<Rightarrow> ('a,'b,'c) com \<Rightarrow> 'b \<Rightarrow> bool"
-  ("\<langle>_,_\<rangle> \<rightarrow>\<^sup>*_ \<langle>_,_\<rangle>" [50,40,40] 70)
-  where "\<langle>c,m\<rangle> \<rightarrow>\<^sup>*t \<langle>c',m'\<rangle> \<equiv> trace_mem m t m' \<and> c \<mapsto>\<^sup>*t c'"
-
-text \<open> Noninterference over all basic commands \<close>
-
-definition sec_pres :: "('a,'b,'c) com \<Rightarrow> 'b rel \<Rightarrow> bool"
-  where 
-  "sec_pres c S \<equiv> \<forall>\<alpha> m\<^sub>1 m\<^sub>2 m\<^sub>1'. 
-     \<alpha> \<in> (obs c) \<longrightarrow> m\<^sub>1 \<in> vc \<alpha> \<longrightarrow> (m\<^sub>1,m\<^sub>2) \<in> S \<longrightarrow> (m\<^sub>1,m\<^sub>1') \<in> beh \<alpha> \<longrightarrow> 
-      (\<exists>m\<^sub>2'. (m\<^sub>2,m\<^sub>2') \<in> beh \<alpha>) \<and> 
-      (\<forall>m\<^sub>2'. (m\<^sub>2,m\<^sub>2') \<in> beh \<alpha> \<longrightarrow> (m\<^sub>1',m\<^sub>2') \<in> S)"
-
-text \<open> Noninterference over all traces \<close>
-
-definition secure :: "('a,'b,'c) com \<Rightarrow> 'b set \<Rightarrow> 'b rel \<Rightarrow> bool"
-  where "secure c P S \<equiv> \<forall>m\<^sub>1 m\<^sub>2 c\<^sub>1 t m\<^sub>1'. 
-        m\<^sub>1 \<in> P \<longrightarrow> (m\<^sub>1,m\<^sub>2) \<in> S \<longrightarrow> \<langle>c,m\<^sub>1\<rangle> \<rightarrow>\<^sup>*t \<langle>c\<^sub>1,m\<^sub>1'\<rangle> \<longrightarrow> 
-        (\<exists>m\<^sub>2' c\<^sub>2. \<langle>c,m\<^sub>2\<rangle> \<rightarrow>\<^sup>*t \<langle>c\<^sub>2,m\<^sub>2'\<rangle>) \<and> 
-        (\<forall>m\<^sub>2' c\<^sub>2. \<langle>c,m\<^sub>2\<rangle> \<rightarrow>\<^sup>*t \<langle>c\<^sub>2,m\<^sub>2'\<rangle> \<longrightarrow> (m\<^sub>1',m\<^sub>2') \<in> S)"  
 
 lemma trace_concat [intro]:
   assumes "P\<^sub>1 \<mapsto>\<^sup>*t\<^sub>1 P\<^sub>2"
@@ -65,7 +39,6 @@ lemma trace_preE [elim]:
   obtains P\<^sub>2 where "P\<^sub>1 \<mapsto>\<^sup>*[x] P\<^sub>2" "P\<^sub>2 \<mapsto>\<^sup>*t P\<^sub>3"
   using assms by (metis append.simps(1) append.simps(2) trace_concatE)
 
-
 lemma trace_rule_nil: 
   assumes "c \<mapsto>\<^sup>*[] c'"
   assumes "R,G \<turnstile> P {c} Q"
@@ -73,117 +46,181 @@ lemma trace_rule_nil:
   using assms by (induct c "[] :: ('a,'b) Trace" c') blast+
 
 lemma trace_rule: 
-  assumes "c \<mapsto>\<^sup>*[g] c'"
+  assumes "c \<mapsto>\<^sup>*[\<alpha>] c'"
   assumes "R,G \<turnstile> P {c} Q"
   assumes "P \<noteq> {}"
-  shows "\<exists>\<alpha> M. \<alpha> \<in> obs c \<and> g = beh \<alpha> \<and> P \<subseteq> wp\<^sub>\<alpha> \<alpha> M \<and> R,G \<turnstile> M {c'} Q"
+  shows "\<exists> M. \<alpha> \<in> obs c  \<and> P \<subseteq> wp\<^sub>\<alpha> \<alpha> M \<and> R,G \<turnstile> M {c'} Q"
   using assms 
-proof (induct c "[g]" c' arbitrary: P) 
+proof (induct c "[\<alpha>]" c' arbitrary: P) 
   case (sil c\<^sub>1 c\<^sub>2 c\<^sub>3)
   then show ?case using obs_sil rewrite_ruleI 
     by (meson subsetD)
 next
   case (gex c\<^sub>1 c\<^sub>2 c\<^sub>3)
-  then obtain \<alpha> M where "P \<subseteq> wp\<^sub>\<alpha> \<alpha> M" "guar\<^sub>\<alpha> \<alpha> G" "g = beh \<alpha>" "R,G \<turnstile> M {c\<^sub>2} Q" "\<alpha> \<in> obs c\<^sub>1"
+  then obtain  M where "P \<subseteq> wp\<^sub>\<alpha> \<alpha> M" "guar\<^sub>\<alpha> \<alpha> G"  "R,G \<turnstile> M {c\<^sub>2} Q" "\<alpha> \<in> obs c\<^sub>1"
     using gexecute_ruleI[OF gex(3,1,4)] by blast
   then show ?case 
     using trace_rule_nil[of c\<^sub>2 c\<^sub>3 R G M Q] gex(2) by blast
 qed
 
-lemma trace_obs:
-  assumes "c\<^sub>1  \<mapsto>\<^sup>*t c\<^sub>2"
-  shows "obs c\<^sub>1 \<supseteq> obs c\<^sub>2"
-  using assms obs_sil obs_gex by induct blast+
+inductive trace_mem :: "'m \<Rightarrow> ('a,'m) Trace  \<Rightarrow> 'm \<Rightarrow> bool" 
+  where
+    [intro]: "trace_mem m [] m" |
+    [intro]: "(m'', m) \<in> beh g \<Longrightarrow> trace_mem m t m' \<Longrightarrow> trace_mem m'' (g#t) m'"
+
+definition ev :: "('a,'b,'c) com \<Rightarrow> 'b \<Rightarrow> ('a,'b) Trace \<Rightarrow> ('a,'b,'c) com \<Rightarrow> 'b \<Rightarrow> bool"
+  ("\<langle>_,_\<rangle> \<rightarrow>\<^sup>*_ \<langle>_,_\<rangle>" [50,40,40] 70)
+  where "\<langle>c,m\<rangle> \<rightarrow>\<^sup>*t \<langle>c',m'\<rangle> \<equiv> trace_mem m t m' \<and> c \<mapsto>\<^sup>*t c'"
+
+text \<open> Noninterference over all traces \<close>
+
+definition secure :: "('a,'b,'c) com \<Rightarrow> 'b set \<Rightarrow> 'b rel \<Rightarrow> ('a,'b) Trace rel \<Rightarrow> bool"
+  where "secure c P S T \<equiv> \<forall>m\<^sub>1 m\<^sub>2 c\<^sub>1 t m\<^sub>1'. 
+        m\<^sub>1 \<in> P \<longrightarrow> m\<^sub>2 \<in> P \<longrightarrow> (m\<^sub>1,m\<^sub>2) \<in> S \<longrightarrow> \<langle>c,m\<^sub>1\<rangle> \<rightarrow>\<^sup>*t \<langle>c\<^sub>1,m\<^sub>1'\<rangle> \<longrightarrow> 
+        (\<exists>m\<^sub>2' c\<^sub>2 t'. (t,t') \<in> T \<and> \<langle>c,m\<^sub>2\<rangle> \<rightarrow>\<^sup>*t' \<langle>c\<^sub>2,m\<^sub>2'\<rangle>) \<and> 
+        (\<forall>m\<^sub>2' c\<^sub>2 t'. (t,t') \<in> T \<longrightarrow> \<langle>c,m\<^sub>2\<rangle> \<rightarrow>\<^sup>*t' \<langle>c\<^sub>2,m\<^sub>2'\<rangle> \<longrightarrow> (m\<^sub>1',m\<^sub>2') \<in> S)"  
+
+fun trace_rel
+  where 
+    "trace_rel [] [] T = True" |
+    "trace_rel (a#t) (b#s) T = ( (a,b) \<in> T \<and> trace_rel t s T)" |
+    "trace_rel _ _ _ = False"
+
+lemma [simp]:
+  "trace_rel [] s T = (s = [])"
+  by (cases s ; auto)
+
+lemma [simp]:
+  "trace_rel (a#t) s T = (\<exists>b tr. s = b#tr \<and> (a,b) \<in> T \<and> trace_rel t tr T)"
+  by (cases s; auto)
+
+text \<open>Low-equivalence structure for a basic operation\<close>
+definition le_basic :: "('a,'b) basic \<Rightarrow> ('a,'b) basic  \<Rightarrow> 'b rel \<Rightarrow> bool"
+  where
+  "le_basic \<alpha> \<beta> R\<^sub>m \<equiv> \<forall>m\<^sub>1 m\<^sub>2 m\<^sub>1'. 
+      m\<^sub>1 \<in> vc \<alpha> \<longrightarrow> m\<^sub>2 \<in> vc \<beta> \<longrightarrow> (m\<^sub>1,m\<^sub>2) \<in> R\<^sub>m \<longrightarrow> (m\<^sub>1,m\<^sub>1') \<in> beh \<alpha> \<longrightarrow> 
+      (\<exists>m\<^sub>2'. (m\<^sub>2,m\<^sub>2') \<in> beh \<beta>) \<and> (\<forall>m\<^sub>2'. (m\<^sub>2,m\<^sub>2') \<in> beh \<beta> \<longrightarrow> (m\<^sub>1',m\<^sub>2') \<in> R\<^sub>m)"
+
+text \<open>Low-equivalence structure for a command\<close>
+definition le_com :: "('a,'b,'c) com rel \<Rightarrow> ('a,'b) basic rel \<Rightarrow> bool"
+  where 
+  "le_com S R \<equiv> \<forall>c\<^sub>1 c\<^sub>2 \<alpha> c\<^sub>1'. (c\<^sub>1, c\<^sub>2) \<in> S \<longrightarrow> c\<^sub>1 \<mapsto>\<^sup>*[\<alpha>] c\<^sub>1' \<longrightarrow>
+      (\<exists>\<beta> c\<^sub>2'. c\<^sub>2 \<mapsto>\<^sup>*[\<beta>] c\<^sub>2' \<and> (\<alpha>,\<beta>) \<in> R \<and> (c\<^sub>1', c\<^sub>2') \<in> S)"
 
 lemma bisim_exists:
-  assumes "sec_pres c S"
-  assumes "R,G \<turnstile> P {c} Q"
-  assumes "(m\<^sub>1,m\<^sub>2) \<in> S"
-  assumes "\<langle>c,m\<^sub>1\<rangle> \<rightarrow>\<^sup>*t \<langle>c\<^sub>1,m\<^sub>1'\<rangle>"
-  assumes "m\<^sub>1 \<in> P"
-  obtains c\<^sub>2 m\<^sub>2' where "\<langle>c,m\<^sub>2\<rangle> \<rightarrow>\<^sup>*t \<langle>c\<^sub>2,m\<^sub>2'\<rangle>" 
-  using assms unfolding ev_def
+  assumes "R,G \<turnstile> P\<^sub>1 {c\<^sub>1} Q"
+  assumes "R,G \<turnstile> P\<^sub>2 {c\<^sub>2} Q"
+  assumes "(m\<^sub>1,m\<^sub>2) \<in> R\<^sub>m"
+  assumes "\<langle>c\<^sub>1,m\<^sub>1\<rangle> \<rightarrow>\<^sup>*t \<langle>c\<^sub>1',m\<^sub>1'\<rangle>"
+  assumes "m\<^sub>1 \<in> P\<^sub>1"
+  assumes "m\<^sub>2 \<in> P\<^sub>2"
+  assumes "(c\<^sub>1,c\<^sub>2) \<in> R\<^sub>c"
+
+  assumes com: "le_com R\<^sub>c R\<^sub>\<alpha>"
+  assumes basic: "R\<^sub>\<alpha> \<subseteq> {(\<alpha>,\<beta>). le_basic \<alpha> \<beta> R\<^sub>m}"
+  obtains c\<^sub>2' m\<^sub>2' t' where "\<langle>c\<^sub>2,m\<^sub>2\<rangle> \<rightarrow>\<^sup>*t' \<langle>c\<^sub>2',m\<^sub>2'\<rangle>" "trace_rel t t' R\<^sub>\<alpha>"
+  using assms(1-7) unfolding ev_def
 proof safe
-  assume "trace_mem m\<^sub>1 t m\<^sub>1'" "sec_pres c S" 
-    "R,G \<turnstile> P {c} Q" "(m\<^sub>1,m\<^sub>2) \<in> S" "c \<mapsto>\<^sup>*t c\<^sub>1" "m\<^sub>1 \<in> P"
-  hence "\<exists>m\<^sub>2' c\<^sub>2. (trace_mem m\<^sub>2 t m\<^sub>2' \<and> c \<mapsto>\<^sup>*t c\<^sub>2) "
-  proof (induct m\<^sub>1 t m\<^sub>1' arbitrary: P m\<^sub>2 c rule: trace_mem.induct)
+  assume "trace_mem m\<^sub>1 t m\<^sub>1'" 
+    "R,G \<turnstile> P\<^sub>1 {c\<^sub>1} Q" "R,G \<turnstile> P\<^sub>2 {c\<^sub>2} Q" "(m\<^sub>1,m\<^sub>2) \<in> R\<^sub>m" "c\<^sub>1 \<mapsto>\<^sup>*t c\<^sub>1'" "m\<^sub>1 \<in> P\<^sub>1" "m\<^sub>2 \<in> P\<^sub>2" "(c\<^sub>1,c\<^sub>2) \<in> R\<^sub>c"
+  hence "\<exists>m\<^sub>2' c\<^sub>2' t'. (trace_mem m\<^sub>2 t' m\<^sub>2' \<and> c\<^sub>2 \<mapsto>\<^sup>*t' c\<^sub>2' \<and> trace_rel t t' R\<^sub>\<alpha>) "
+  proof (induct m\<^sub>1 t m\<^sub>1' arbitrary: P\<^sub>1 P\<^sub>2 m\<^sub>2 c\<^sub>2 c\<^sub>1 rule: trace_mem.induct)
     case (1 m)
-    then show ?case by blast
+    then show ?case by simp blast
   next
-    case (2 m\<^sub>1 m\<^sub>1' g t m\<^sub>1'')
-    then obtain c' where itm1: "c \<mapsto>\<^sup>*[g] c'" "c' \<mapsto>\<^sup>*t c\<^sub>1" by auto
-    then obtain P' \<alpha>  where itm2: 
-        "R,G \<turnstile> P' {c'} Q" "\<alpha> \<in> obs c" "g = beh \<alpha>" "P \<subseteq> wp\<^sub>\<alpha> \<alpha> P'"  
-      using trace_rule[OF itm1(1) 2(5)] 2(8) 
-      by (metis empty_iff)
-    hence itm6: "m\<^sub>1' \<in> P'" using 2(1,8) unfolding wp_def by blast                       
-    then obtain m\<^sub>2' where itm3: "(m\<^sub>2,m\<^sub>2') \<in> g" "(m\<^sub>1',m\<^sub>2') \<in> S" using 2(1,4,6,8) itm2(2,3,4) 
-      unfolding sec_pres_def wp_def by blast
-    hence itm4: "sec_pres c' S" 
-      using 2(4) itm1 itm2(2) trace_obs unfolding sec_pres_def by blast
-    hence itm5: "\<exists>m\<^sub>2'' c\<^sub>2. (trace_mem m\<^sub>2' t m\<^sub>2'' \<and> c' \<mapsto>\<^sup>*t c\<^sub>2)"
-      using 2(3)[OF itm4 itm2(1) itm3(2) itm1(2) itm6] by blast
-    then show ?case using "2.prems"(4) itm3(1) by blast
+    case (2 m\<^sub>1 m\<^sub>1' \<alpha> t m\<^sub>1'')
+    then obtain c' where \<alpha>: "c\<^sub>1 \<mapsto>\<^sup>*[\<alpha>] c'" "c' \<mapsto>\<^sup>*t c\<^sub>1'" by auto
+    then obtain P\<^sub>1' where itm1: "R,G \<turnstile> P\<^sub>1' {c'} Q" "P\<^sub>1 \<subseteq> wp\<^sub>\<alpha> \<alpha> P\<^sub>1'"  
+      using trace_rule[OF \<alpha>(1) 2(4)] 2(8) by (metis empty_iff)
+    hence m1': "m\<^sub>1' \<in> P\<^sub>1'" using 2(1,8) unfolding wp_def by blast
+    have m1: "m\<^sub>1 \<in> vc \<alpha>" using itm1 2 by (simp add: subset_eq wp_def) 
+
+    then obtain \<beta> c\<^sub>2' where \<beta>: "c\<^sub>2 \<mapsto>\<^sup>*[\<beta>] c\<^sub>2'" "(\<alpha>,\<beta>) \<in> R\<^sub>\<alpha>" "(c', c\<^sub>2') \<in> R\<^sub>c"
+      using com 2(10) \<alpha> unfolding le_com_def by blast
+    then obtain P\<^sub>2' where itm2: "R,G \<turnstile> P\<^sub>2' {c\<^sub>2'} Q" "P\<^sub>2 \<subseteq> wp\<^sub>\<alpha> \<beta> P\<^sub>2'"  
+      using trace_rule[OF \<beta>(1) 2(5)] 2(9) by (metis empty_iff)
+    have m2: "m\<^sub>2 \<in> vc \<beta>" using itm2 2 by (simp add: subset_eq wp_def) 
+
+    then obtain m\<^sub>2' where itm3: "(m\<^sub>2,m\<^sub>2') \<in> beh \<beta>" "(m\<^sub>1', m\<^sub>2') \<in> R\<^sub>m"
+      using m1 \<beta> basic 2(1,6) unfolding le_basic_def by blast
+    hence m2': "m\<^sub>2' \<in> P\<^sub>2'" using itm2 2(1,9) unfolding wp_def by blast
+
+    hence itm4: "\<exists>m\<^sub>2'' c\<^sub>2'' t'. (trace_mem m\<^sub>2' t' m\<^sub>2'' \<and> c\<^sub>2' \<mapsto>\<^sup>*t' c\<^sub>2'' \<and> trace_rel t t' R\<^sub>\<alpha>)"
+      using 2(3)[OF itm1(1) itm2(1) itm3(2) \<alpha>(2) m1' m2' \<beta>(3)] by blast
+
+    then show ?case using itm3(1) \<beta>(1,2) 
+      by (smt (verit) append_Cons trace_concat  self_append_conv2 trace_mem.intros(2) trace_rel.simps(2))
   qed
   thus ?thesis using that by (meson ev_def)
 qed
 
 lemma bisim_all:
-  assumes "sec_pres c\<^sub>1 S"
-  assumes "R,G \<turnstile> P {c\<^sub>1} Q"
-  assumes "R,G \<turnstile> P {c\<^sub>2} Q"
-  assumes "(m\<^sub>1,m\<^sub>2) \<in> S"
+  assumes "R,G \<turnstile> P\<^sub>1 {c\<^sub>1} Q"
+  assumes "R,G \<turnstile> P\<^sub>2 {c\<^sub>2} Q"
+  assumes "(m\<^sub>1,m\<^sub>2) \<in> R\<^sub>m"
   assumes "\<langle>c\<^sub>1,m\<^sub>1\<rangle> \<rightarrow>\<^sup>*t \<langle>c\<^sub>1',m\<^sub>1'\<rangle>"
-  assumes "\<langle>c\<^sub>2,m\<^sub>2\<rangle> \<rightarrow>\<^sup>*t \<langle>c\<^sub>2',m\<^sub>2'\<rangle>"
-  assumes "m\<^sub>1 \<in> P"
-  shows "(m\<^sub>1', m\<^sub>2') \<in> S"
-  using assms unfolding ev_def
+  assumes "\<langle>c\<^sub>2,m\<^sub>2\<rangle> \<rightarrow>\<^sup>*t' \<langle>c\<^sub>2',m\<^sub>2'\<rangle>"
+  assumes "m\<^sub>1 \<in> P\<^sub>1"
+  assumes "m\<^sub>2 \<in> P\<^sub>2"
+  assumes "trace_rel t t' R\<^sub>\<alpha>"
+
+  assumes basic: "R\<^sub>\<alpha> \<subseteq> {(\<alpha>,\<beta>). le_basic \<alpha> \<beta> R\<^sub>m}"
+  shows "(m\<^sub>1', m\<^sub>2') \<in> R\<^sub>m"
+  using assms(1-8) unfolding ev_def
 proof safe
-  assume "trace_mem m\<^sub>1 t m\<^sub>1'" "trace_mem m\<^sub>2 t m\<^sub>2'" "sec_pres c\<^sub>1 S" 
-    "R,G \<turnstile> P {c\<^sub>1} Q" "R,G \<turnstile> P {c\<^sub>2} Q" "(m\<^sub>1,m\<^sub>2) \<in> S" "c\<^sub>1 \<mapsto>\<^sup>*t c\<^sub>1'" "c\<^sub>2 \<mapsto>\<^sup>*t c\<^sub>2'" "m\<^sub>1 \<in> P"
-  hence "(m\<^sub>1', m\<^sub>2') \<in> S"
-  proof (induct m\<^sub>1 t m\<^sub>1' arbitrary: P m\<^sub>2 c\<^sub>1 c\<^sub>2 rule: trace_mem.induct)
+  assume "trace_mem m\<^sub>1 t m\<^sub>1'" "trace_mem m\<^sub>2 t' m\<^sub>2'" 
+    "R,G \<turnstile> P\<^sub>1 {c\<^sub>1} Q" "R,G \<turnstile> P\<^sub>2 {c\<^sub>2} Q" "(m\<^sub>1,m\<^sub>2) \<in> R\<^sub>m" "c\<^sub>1 \<mapsto>\<^sup>*t c\<^sub>1'" "c\<^sub>2 \<mapsto>\<^sup>*t' c\<^sub>2'" "m\<^sub>1 \<in> P\<^sub>1" "m\<^sub>2 \<in> P\<^sub>2"
+    "trace_rel t t' R\<^sub>\<alpha>" 
+  hence "(m\<^sub>1', m\<^sub>2') \<in> R\<^sub>m"
+  proof (induct m\<^sub>1 t m\<^sub>1' arbitrary: t' P\<^sub>1 P\<^sub>2 m\<^sub>2 c\<^sub>1 c\<^sub>2 rule: trace_mem.induct)
     case (1 m)
-    then show ?case by (auto elim: trace_mem.cases)
+    then show ?case using 1 by (auto elim: trace_mem.cases)
   next
-    case (2 m\<^sub>1 m\<^sub>1'' g t m\<^sub>1')
-    then obtain c\<^sub>1'' where itm1: "c\<^sub>1 \<mapsto>\<^sup>*[g] c\<^sub>1''" "c\<^sub>1'' \<mapsto>\<^sup>*t c\<^sub>1'" by auto
-    then obtain c\<^sub>2'' where itm2: "c\<^sub>2 \<mapsto>\<^sup>*[g] c\<^sub>2''" "c\<^sub>2'' \<mapsto>\<^sup>*t c\<^sub>2'" using 2 by auto
-    then obtain m\<^sub>2'' where itm3: "(m\<^sub>2, m\<^sub>2'') \<in> g" "trace_mem m\<^sub>2'' t m\<^sub>2'"
-      using 2(4) by (auto elim: trace_mem.cases)
+    case (2 m\<^sub>1 m\<^sub>1'' \<alpha> t m\<^sub>1')
+    then obtain \<beta> tr where t: "t' = \<beta>#tr" "(\<alpha>, \<beta>) \<in> R\<^sub>\<alpha>" "trace_rel t tr R\<^sub>\<alpha>" by auto
+    then obtain c\<^sub>1'' where itm1: "c\<^sub>1 \<mapsto>\<^sup>*[\<alpha>] c\<^sub>1''" "c\<^sub>1'' \<mapsto>\<^sup>*t c\<^sub>1'" using 2 by auto
+    then obtain c\<^sub>2'' where itm2: "c\<^sub>2 \<mapsto>\<^sup>*[\<beta>] c\<^sub>2''" "c\<^sub>2'' \<mapsto>\<^sup>*tr c\<^sub>2'" using 2 t by blast 
+    then obtain m\<^sub>2'' where itm3: "(m\<^sub>2, m\<^sub>2'') \<in> beh \<beta>" "trace_mem m\<^sub>2'' tr m\<^sub>2'"
+      using 2(4) t by (metis list.distinct(1) list.inject trace_mem.cases)  
 
-    then obtain P\<^sub>1 \<alpha>  where itm4: 
-        "R,G \<turnstile> P\<^sub>1 {c\<^sub>1''} Q" "\<alpha> \<in> obs c\<^sub>1" "g = beh \<alpha>" "P \<subseteq> wp\<^sub>\<alpha> \<alpha> P\<^sub>1"  
-      using trace_rule[OF itm1(1) 2(6)] 2(11) by blast
-    then obtain P\<^sub>2 \<beta>  where itm5: 
-        "R,G \<turnstile> P\<^sub>2 {c\<^sub>2''} Q" "\<beta> \<in> obs c\<^sub>2" "g = beh \<beta>" "P \<subseteq> wp\<^sub>\<alpha> \<beta> P\<^sub>2"  
-      using trace_rule[OF itm2(1) 2(7)] 2(11) by blast
+    obtain P\<^sub>1' where itm4: "R,G \<turnstile> P\<^sub>1' {c\<^sub>1''} Q" "P\<^sub>1 \<subseteq> wp\<^sub>\<alpha> \<alpha> P\<^sub>1'"  
+      using trace_rule[OF itm1(1) 2(5)] 2(10) by blast
+    then obtain P\<^sub>2' where itm5: "R,G \<turnstile> P\<^sub>2' {c\<^sub>2''} Q" "P\<^sub>2 \<subseteq> wp\<^sub>\<alpha> \<beta> P\<^sub>2'"  
+      using trace_rule[OF itm2(1) 2(6)] 2(11) by blast
 
-    have j: "R,G \<turnstile> P\<^sub>1 \<inter> P\<^sub>2 {c\<^sub>1''} Q" "R,G \<turnstile> P\<^sub>1 \<inter> P\<^sub>2 {c\<^sub>2''} Q"
-      using itm4 itm5 by auto
+    have m1: "m\<^sub>1 \<in> vc \<alpha>" using itm4 2 by (simp add: subset_eq wp_def) 
+    have m2: "m\<^sub>2 \<in> vc \<beta>" using itm5 2 by (simp add: subset_eq wp_def) 
 
-    have a: "(m\<^sub>1'', m\<^sub>2'') \<in> S"
-      using 2 itm4 itm5
-      unfolding sec_pres_def wp_def
-      by (smt (verit, del_insts) Int_iff itm3(1) subset_eq)
-    have b: "m\<^sub>1'' \<in> P\<^sub>1 \<inter> P\<^sub>2" 
-      by (smt (verit) "2.hyps"(1) "2.prems"(8) Int_Collect Int_iff itm4(3,4) itm5(3,4) subset_eq wp_def)
-    have c: "sec_pres c\<^sub>1'' S" 
-      by (smt (verit, ccfv_SIG) "2.prems"(2) itm1(1) sec_pres_def subset_eq trace_obs)
-
-    show ?case using 2(3)[OF itm3(2) c j a itm1(2) itm2(2) b] .
+    have a: "(m\<^sub>1'', m\<^sub>2'') \<in> R\<^sub>m" using basic t(2) 2(1,7) itm3(1) m1 m2 unfolding le_basic_def
+      by blast
+    have b: "m\<^sub>1'' \<in> P\<^sub>1'" "m\<^sub>2'' \<in> P\<^sub>2'" 
+      using itm4(2) itm5(2) 2(10,11) itm3(1) 2(1) sp_def sp_wp by fastforce+
+    show ?case using 2(3)[OF itm3(2) itm4(1) itm5(1) a itm1(2) itm2(2) b t(3)] .
   qed
   thus ?thesis .
 qed
 
 theorem secure_bisim:
   assumes "R,G \<turnstile> P { c } Q"
-  assumes "sec_pres c S"
-  shows "secure c P S"
-  using bisim_exists[OF assms(2) assms(1)]
-  using bisim_all[OF assms(2) assms(1) assms(1)]
-  unfolding secure_def by metis
+  assumes "refl R\<^sub>c"
+  assumes "le_com R\<^sub>c R\<^sub>\<alpha>"
+  assumes "R\<^sub>\<alpha> \<subseteq> {(\<alpha>, \<beta>). le_basic \<alpha> \<beta> R\<^sub>m}"
+  shows "secure c P R\<^sub>m {(t,t'). trace_rel t t' R\<^sub>\<alpha>}"
+  unfolding secure_def
+proof (intro allI impI conjI)
+  fix m\<^sub>1 m\<^sub>2 c\<^sub>1 t m\<^sub>1'
+  assume a: "m\<^sub>1 \<in> P" "m\<^sub>2 \<in> P" "(m\<^sub>1, m\<^sub>2) \<in> R\<^sub>m" "\<langle>c,m\<^sub>1\<rangle> \<rightarrow>\<^sup>*t \<langle>c\<^sub>1,m\<^sub>1'\<rangle>"
+  show "(\<exists>m\<^sub>2' c\<^sub>2 t'.
+           (t, t') \<in> {(t, t'). trace_rel t t' R\<^sub>\<alpha>} \<and>
+           \<langle>c,m\<^sub>2\<rangle> \<rightarrow>\<^sup>*t' \<langle>c\<^sub>2,m\<^sub>2'\<rangle>)"
+    using bisim_exists[OF assms(1) assms(1) a(3,4,1,2) _ assms(3,4)]
+    using assms(2) reflD by fastforce 
+next
+  fix m\<^sub>1 m\<^sub>2 c\<^sub>1 t m\<^sub>1' m\<^sub>2' c\<^sub>2 t'
+  assume a: "m\<^sub>1 \<in> P" "m\<^sub>2 \<in> P" "(m\<^sub>1, m\<^sub>2) \<in> R\<^sub>m" "\<langle>c,m\<^sub>1\<rangle> \<rightarrow>\<^sup>*t \<langle>c\<^sub>1,m\<^sub>1'\<rangle>" 
+            "(t, t') \<in> {(t, t'). trace_rel t t' R\<^sub>\<alpha>}" " \<langle>c,m\<^sub>2\<rangle> \<rightarrow>\<^sup>*t' \<langle>c\<^sub>2,m\<^sub>2'\<rangle>"
+  thus "(m\<^sub>1', m\<^sub>2') \<in> R\<^sub>m" using bisim_all assms(1,4) by blast
+qed
 
 end
 
